Compatibility with bumped rewriter
This is in preparation for having typedefs based on bounds info.

If this passes CI, then we can merge
https://github.com/mit-plv/rewriter/pull/28.

src/AbstractInterpretation/ZRange.v
@@ -43,7 +43,7 @@ Module Compilers.
              | base.type.type_base base.type.Z => is_tighter_than_bool
              | base.type.type_base _ as t
              | base.type.unit as t
-               => base.interp_beq (@base.base_interp_beq)
+               => base.interp_beq (fun t => @base.base_interp_beq t t)
              | base.type.prod A B
                => fun '(a, b) '(a', b')
                   => @is_tighter_than A a a' && @is_tighter_than B b b'
@@ -57,7 +57,7 @@ Module Compilers.
              | base.type.type_base base.type.Z => fun r z => ZRange.is_bounded_by_bool z r
              | base.type.type_base _ as t
              | base.type.unit as t
-               => base.interp_beq (@base.base_interp_beq)
+               => base.interp_beq (fun t => @base.base_interp_beq t t)
              | base.type.prod A B
                => fun '(a, b) '(a', b')
                   => @is_bounded_by A a a' && @is_bounded_by B b b'
@@ -66,29 +66,36 @@ Module Compilers.
              | base.type.option A
                => option_beq_hetero (@is_bounded_by A)
              end.
-        Fixpoint interp_beq {t} : interp t -> interp t -> bool
-          := match t return interp t -> interp t -> bool with
-             | base.type.type_base base.type.Z => zrange_beq
-             | base.type.type_base _ as t
-             | base.type.unit as t
-               => base.interp_beq (@base.base_interp_beq)
-             | base.type.prod A B
+        Fixpoint interp_beq {t1 t2} : interp t1 -> interp t2 -> bool
+          := match t1, t2 return interp t1 -> interp t2 -> bool with
+             | base.type.type_base base.type.Z, base.type.type_base base.type.Z => zrange_beq
+             | base.type.type_base base.type.Z, _ | _, base.type.type_base base.type.Z => fun _ _ => false
+             | base.type.type_base _ as t1, base.type.type_base _ as t2
+             | base.type.unit as t1, base.type.unit as t2
+               => base.interp_beq_hetero (@base.base_interp_beq)
+             | base.type.prod A1 B1, base.type.prod A2 B2
                => fun '(a, b) '(a', b')
-                  => @interp_beq A a a' && @interp_beq B b b'
-             | base.type.list A
-               => list_beq _ (@interp_beq A)
-             | base.type.option A
-               => option_beq (@interp_beq A)
+                  => @interp_beq A1 A2 a a' && @interp_beq B1 B2 b b'
+             | base.type.list A1, base.type.list A2
+               => list_beq_hetero (@interp_beq A1 A2)
+             | base.type.option A1, base.type.option A2
+               => option_beq_hetero (@interp_beq A1 A2)
+             | base.type.type_base _, _
+             | base.type.unit, _
+             | base.type.prod _ _, _
+             | base.type.list _, _
+             | base.type.option _, _
+               => fun _ _ => false
              end%bool.
 
-        Global Instance reflect_interp_eq {t} : reflect_rel (@eq _) (@interp_beq t).
+        Global Instance reflect_interp_eq {t} : reflect_rel (@eq _) (@interp_beq t t).
         Proof.
           induction t; cbn [interp_beq]; intros; break_innermost_match; try exact _.
         Defined.
 
-        Lemma interp_beq_bl {t x y} : @interp_beq t x y = true -> x = y.
+        Lemma interp_beq_bl {t x y} : @interp_beq t t x y = true -> x = y.
         Proof. apply reflect_to_beq; exact _. Qed.
-        Lemma interp_beq_lb {t x y} : x = y -> @interp_beq t x y = true.
+        Lemma interp_beq_lb {t x y} : x = y -> @interp_beq t t x y = true.
         Proof. apply reflect_to_beq; exact _. Qed.
 
         Module option.
@@ -142,6 +149,17 @@ Module Compilers.
                | base.type.prod A B
                  => fun '(a, b) => a <- @lift_Some A a; b <- @lift_Some B b; Datatypes.Some (a, b)
                end%option.
+          Fixpoint is_informative {t} : interp t -> bool (* true iff there's some bounds info *)
+            := match t with
+               | base.type.type_base _
+               | base.type.list _
+               | base.type.option _
+                 => Option.is_Some
+               | base.type.unit
+                 => fun _ => false
+               | base.type.prod A B
+                 => fun '(a, b) => orb (@is_informative A a) (@is_informative B b)
+               end.
           (** Keep data about list length and nat value, but not zrange *)
           Fixpoint strip_ranges {t} : interp t -> interp t
             := match t with
@@ -196,27 +214,33 @@ Module Compilers.
                        end
                | base.type.unit => fun 'tt 'tt => true
                end.
-          Fixpoint interp_beq {t} : interp t -> interp t -> bool
-            := match t return interp t -> interp t -> bool with
-               | base.type.type_base _ as t => option_beq base.interp_beq
-               | base.type.prod A B
+          Fixpoint interp_beq {t1 t2} : interp t1 -> interp t2 -> bool
+            := match t1, t2 return interp t1 -> interp t2 -> bool with
+               | base.type.type_base _ as t1, base.type.type_base _ as t2 => option_beq_hetero base.interp_beq
+               | base.type.prod A1 B1, base.type.prod A2 B2
                  => fun '(a, b) '(a', b')
-                    => @interp_beq A a a' && @interp_beq B b b'
-               | base.type.list A
-                 => option_beq (list_beq _ (@interp_beq A))
-               | base.type.option A
-                 => option_beq (option_beq (@interp_beq A))
-               | base.type.unit => fun 'tt 'tt => true
+                    => @interp_beq A1 A2 a a' && @interp_beq B1 B2 b b'
+               | base.type.list A1, base.type.list A2
+                 => option_beq_hetero (list_beq_hetero (@interp_beq A1 A2))
+               | base.type.option A1, base.type.option A2
+                 => option_beq_hetero (option_beq_hetero (@interp_beq A1 A2))
+               | base.type.unit, base.type.unit => fun 'tt 'tt => true
+               | base.type.type_base _, _
+               | base.type.unit, _
+               | base.type.prod _ _, _
+               | base.type.list _, _
+               | base.type.option _, _
+                 => fun _ _ => false
                end.
 
-          Global Instance reflect_interp_eq {t} : reflect_rel (@eq _) (@interp_beq t).
+          Global Instance reflect_interp_eq {t} : reflect_rel (@eq _) (@interp_beq t t).
           Proof.
             induction t; cbn [interp_beq]; intros; break_innermost_match; try exact _.
           Defined.
 
-          Lemma interp_beq_bl {t x y} : @interp_beq t x y = true -> x = y.
+          Lemma interp_beq_bl {t x y} : @interp_beq t t x y = true -> x = y.
           Proof. apply reflect_to_beq; exact _. Qed.
-          Lemma interp_beq_lb {t x y} : x = y -> @interp_beq t x y = true.
+          Lemma interp_beq_lb {t x y} : x = y -> @interp_beq t t x y = true.
           Proof. apply reflect_to_beq; exact _. Qed.
 
           Fixpoint is_bounded_by {t} : interp t -> binterp t -> bool
